progress - maybe

dfy/cnf.dfy
@@ -6,7 +6,8 @@ include "sat.dfy"
 module CNF {
     import opened SAT
 
-function clause_literal_count(c: Clause) : int
+function clause_literal_count(c: Clause) : (out: int)
+    ensures out >= 0
 {
     |c|
 }
@@ -20,9 +21,13 @@ function clause_is_tautology(c: Clause) : (out: bool)
 }
 
 
-method cnf_literal_count(cnf: CNF) returns (out: int)
+function cnf_literal_count(cnf: CNF) : (out: int)
+    ensures out >= 0
 {
-    out := Util.set_sum(set c | c in cnf :: clause_literal_count(c));
+    var cnts := map c | c in cnf :: clause_literal_count(c);
+    Util.map_sum(cnts)
+    // Util.NonNegativesSumToNonNegative(cnts);
+    // Util.set_sum(cnts)
 }
 
 ghost function cnf_equivalent(cnf: CNF, other: CNF) : (eq: bool)
@@ -77,6 +82,7 @@ function merge_resolution(v: Variable, c1: Clause, c2: Clause) : (out: Clause)
     requires NotInverted(v) in c1 && Inverted(v) in c2
     ensures cnf_implies({c1, c2}, {out})
     ensures forall cnf : CNF :: c1 in cnf && c2 in cnf ==> cnf_implies(cnf, cnf - {c1, c2} + {out})
+    ensures clause_literal_count(out) < clause_literal_count(c1) + clause_literal_count(c2)
 {
     ghost var example := map[v := true];
     assert v in example;
@@ -91,62 +97,44 @@ method cnf_some_resolution(cnf: CNF) returns (v: Variable, c1: Clause, c2: Claus
     v, c1, c2 :| v in cnf_vars(cnf) && c1 in cnf && c2 in cnf && cnf_has_resolution_with(cnf, v, c1, c2);
 }
 
-// lemma SetWithSomethingInItIsNotEmpty<T>(s: set<T>, f: T -> bool, ss: set<T>)
-//     requires exists x :: x in s && f(x)
-//     requires ss == set x | x in s && f(x)
-//     ensures |ss| > 0
-// {
-//     var x :| x in s && f(x);
-//     assert x in s;
-//     assert f(x);
-//     assert x in ss;
-//     assert |ss| > 0;
-// }
-
 method cnf_resolution_step(cnf: CNF) returns (out: CNF)
     requires !cnf_has_tautologies(cnf)
     requires cnf_has_resolution(cnf)
+    ensures !cnf_has_tautologies(out)
     ensures cnf_implies(cnf, out)
-    ensures |out| < |cnf|
+    ensures cnf_literal_count(out) < cnf_literal_count(cnf)
 {
     var v,c1,c2 := cnf_some_resolution(cnf);
     assert NotInverted(v) in c1;
     assert c1 != c2;
     var merged := merge_resolution(v, c1, c2);
+
+    out := cnf - {c1, c2} + {merged};
+    assert cnf_implies(cnf, out);
+    assert clause_literal_count(merged) < clause_literal_count(c1) + clause_literal_count(c2);
     assume false;
 
-    assert c1 != merged;
-    assert c2 != merged;
-    out := cnf - {c1, c2} + {merged};
+    assert cnf_literal_count(out) == cnf_literal_count(cnf) - clause_literal_count(c1) - clause_literal_count(c2) + clause_literal_count(merged);
 }
 
-// function cnf_resolution(cnf: CNF) : (out: CNF)
+// method cnf_resolution(cnf: CNF) returns (out: CNF)
 //     requires !cnf_has_tautologies(cnf)
-//     requires cnf_has_resolution(cnf)
-//     ensures cnf_equivalent(cnf, out)
+//     ensures !cnf_has_resolution(cnf)
+//     ensures cnf_implies(cnf, out)
 // {
-//     var v := cnf_some_resolution_var(cnf);
-//     assert exists l1, l2, c1, c2 ::
-//         c1 in cnf && c2 in cnf && c1 != c2 &&
-//         l1 in c1 && NotInverted(v) == l1 &&
-//         l2 in c2 && Inverted(v) == l2;
-//     assert exists c :: c in cnf && NotInverted(v) in c;
+//     out := cnf;
 
-//     var f :=  (c: Clause) => NotInverted(v) in c;
-//     var where_not_inverted: set<Clause> := set c | c in cnf && f(c);
-//     assert exists c :: c in cnf && f(c);
-//     SetSetWithSomethingInItIsNotEmpty(cnf, f, where_not_inverted);
-//     assume false;
-//     assert |where_not_inverted| > 0;
-
-
-//     // var where_inverted: set<Clause> := set c | c in cnf && Inverted(v) in c;
-//     // assert |where_inverted| > 0;
-
-//     // var c1 :| c1 in not_inverted[v];
-//     // var c2 :| c2 in inverted[v];
-
-//     cnf
+//     while cnf_has_resolution(out)
+//         invariant !cnf_has_tautologies(out)
+//         invariant cnf_implies(cnf, out)
+//         decreases cnf_literal_count(out)
+//     {
+//         var out' := cnf_resolution_step(out);
+//         assert cnf_implies(cnf, out);
+//         assert cnf_implies(out, out');
+//         assert cnf_implies(cnf, out');
+//         assert cnf_literal_count(out') < cnf_literal_count(out);
+//     }
 // }
 
 }
